Add the new consistency property accessibleVAIsNotPartitionDescriptor
+ Fix invariants to take into account this new property

+ Prove new internal lemmas required to propagate the new consistency property

+ Use this consistency property on the writeAccessible invariant to prove that the partition descriptor flag of the involved entry is equal to false in case of updating the current partition configuration

proof/StateLib.v
@@ -638,15 +638,17 @@ Definition getTableAddrRoot table idxroot currentPart va s : Prop :=
 Definition getAllPages: list page:= 
 map CPage (seq 0 nbPage ).
 
+(** The [getPDFlag] checks if the given virtual address corresponds to a partition
+    descriptor **)
 Definition getPDFlag sh1 va s :=
-let idxVA := StateLib.getIndexOfAddr va fstLevel in
-match StateLib.getNbLevel with
+let idxVA := getIndexOfAddr va fstLevel in
+match getNbLevel with
 |Some nbL =>  match getIndirection sh1 va nbL (nbLevel - 1) s with
   | Some tbl =>
       if tbl =? defaultPage
       then false
       else
-       match StateLib.readPDflag tbl idxVA (memory s) with
+       match readPDflag tbl idxVA (memory s) with
        | Some true => true
        | Some false => false
        | None => false
@@ -656,4 +658,6 @@ match StateLib.getNbLevel with
 | None => false
 end.
 
-
+Definition isPartitionFalse ptPDChildSh1 idxPDChild s :=
+readPDflag ptPDChildSh1 idxPDChild (memory s) = Some false \/
+readPDflag ptPDChildSh1 idxPDChild (memory s) = None.
